separated AAEnv Env Related Stuff from test set

C11-BackEnds/Clean_wrapper/examples/Coder_Test_ExprStmt.thy
@@ -1,160 +1,7 @@
 theory "Coder_Test_ExprStmt"
-  imports "../src/CleanCoder"
+  imports "../src/CleanCoder" Coder_Test_Env_AEnv
 begin
 
-
-
-section \<open>Accessors to C-Env\<close>
-
-ML\<open>
-fun map_option f (SOME X) = SOME(f X)
-   |map_option f NONE     = NONE   
-
-fun lookup_Cid_info (C_env:C_Module.Data_In_Env.T) id = Symtab.lookup(#idents(#var_table C_env)) id
-
-fun is_global_Cid Cenv Cid     = map_option (#global o #3) (lookup_Cid_info Cenv Cid);
-fun is_fun_Cid Cenv Cid        = map_option ((fn [C_Ast.CFunDeclr0 _] => true | _ => false) 
-                                               o (#params o #3)) 
-                                            (lookup_Cid_info Cenv Cid);
-fun get_CDeclSpecS_Cid Cenv id = map_option (#ret o #3) (lookup_Cid_info Cenv id);
-
-(* Fundsachen *)
-C11_Ast_Lib.encode_positions;
-C11_Ast_Lib.decode_positions;
-C11_Ast_Lib.toString_abr_string;
-C11_Ast_Lib.toString_nodeinfo;
-
-C_Ast.SS_base
-\<close>
-
-section \<open>Global Variables, Local Variables, and Local Parameters\<close>
-subsection\<open>An Environment Spy\<close>
-
-ML\<open>
-val ENV = Unsynchronized.ref (@{C\<^sub>e\<^sub>n\<^sub>v})
-fun print_env' s _ stack _ env thy =
-  let
-    val () = (ENV:=env; writeln ("ENV " ^ C_Env.string_of env))
-  in thy end
-\<close>
-
-ML\<open>open Position\<close>
-setup \<open>ML_Antiquotation.inline @{binding print_env'}
-                               (Scan.peek (fn _ => Scan.option Args.text)
-                                >> (fn name => ("print_env' "
-                                                ^ (case name of NONE => "NONE"
-                                                              | SOME s => "(SOME \"" ^ s ^ "\")")
-                                                ^ " " ^ ML_Pretty.make_string_fn)))\<close>
-
-subsection\<open>Accessing the C_Env in an Example\<close>
-
-C \<comment> \<open>Nesting ML code in C comments\<close> \<open>
-int a(int b){int c; 
-              return c;
-              /*@@ \<approx>setup \<open>@{print_env'}\<close> */
-              /*@@ highlight */
-             }; 
-                 
-\<close>
-
-
-ML\<open>
-val a_res = lookup_Cid_info (!ENV) "a";
-val b_res = lookup_Cid_info (!ENV) "b";
-val c_res = lookup_Cid_info (!ENV) "c"
-\<close>
-
-
-(* Problematic : *)
-C \<comment> \<open>Nesting ML code in C comments\<close> \<open>
-int a (int b){int b; 
-              return b;
-              /*@@ highlight */
-              /*@@ \<approx>setup \<open>@{print_env'}\<close> */}; 
-                 
-\<close>
-ML\<open>
-lookup_Cid_info (!ENV) "a";
-lookup_Cid_info (!ENV) "b"
-\<close>
-
-
-
-
-
-section \<open>Global Declarations via CEnv and via the Clean API\<close>
-
-text \<open>
-First, we translate the expressions;
-we can have binary operators, unary operators, or constants.
-The attributs can be constantes or variables. 
-In order to simulate the use of variables, we construct a "fake" record local_state
-\<close>
-
-global_vars (test)  (*intern label *)
-            a     :: "int"
-
-(* creation of a global variable Clean state with "a" *)
-ML\<open>val Const(longid_a,Type("fun",[sigma_i, _])) = @{term "a"}; \<close>
-
-
-(* creation of two declarations with "a" an array and "f" a function *)
-
-declare [[C\<^sub>r\<^sub>u\<^sub>l\<^sub>e\<^sub>0 = "translation_unit"]]
-declare [[C\<^sub>e\<^sub>n\<^sub>v\<^sub>0 = last]]
-
-C\<open> int a[10+12][34][] = 1;
-   short int f(int x [][], long double y)
-     {int y; x=x;
-      /*@@ \<approx>setup \<open>@{print_env'}\<close> */
-      /*@@ highlight */}
-     ;
-      
-\<close>
-
-(* binding the resulting C_Env to env_expr *)
-
-ML\<open>val env_expr : C_Module.Data_In_Env.T =  @{C\<^sub>e\<^sub>n\<^sub>v};\<close>
-
-(* messing around with the C identifier "a" and "f" in the env AFTER the translation unit*)
-ML\<open>
-   val SOME(pos_list,ser,S)    = lookup_Cid_info env_expr "a";
-   val SOME(pos_list',ser',S') = lookup_Cid_info env_expr "f";
-   val NONE = lookup_Cid_info env_expr "x";
-\<close>
-(* handy decompositions *)
-ML\<open>
-
-local open C_Ast C_Env in
-
-   val [CArrDeclr0 (HH,CArrSize0 (_,CBinary0 X),_),
-        CArrDeclr0 (_,CArrSize0  (_,CConst0 Y), _), 
-        CArrDeclr0 (_,CNoArrSize0 Z,_)] = #params S
-   val [CFunDeclr0 (Right([CDecl0 (A,A' as [((Some (CDeclr0 (_,TT,_,_,_)),_),_)],_),
-                           CDecl0 (B,B' as [((Some (CDeclr0 (_,TT',_,_,_)),_),_)],_)],s), _, _)] 
-       = #params S'
-
-
-val [((Some (CDeclr0 (_,s,_,_,_)),_),_)] = A'
-val [((Some (CDeclr0 (_,t,_,_,_)),_),_)] = B'
-
-end
-\<close>
-
-ML\<open>(#ret o #3 o the)(lookup_Cid_info env_expr "f" );\<close>
-
-ML\<open>
-C11_TypeSpec_2_CleanTyp.conv_CDerivedDecl_typ;C_Ast.CFunDeclr0;
-val S = hd ((#params o  #3 o the)(lookup_Cid_info env_expr "f" ));
-val S' = C11_TypeSpec_2_CleanTyp.conv_CDerivedDecl_typ [S] sigma_i
-\<close>
-(* and the whole thing a bit more abstract with "a" and "f" *)
-ML\<open>
-map_option (C11_TypeSpec_2_CleanTyp.conv_GlobalIdDescr_typ o #3) (lookup_Cid_info env_expr "a" );
-(* map_option (conv_GlobalIdDescr_typ o #3) (lookup_Cid_info env_expr "f" ); *)
-map_option (C11_TypeSpec_2_CleanTyp.conv_GlobalIdDescr_typ o #3) (lookup_Cid_info env_expr "x" );
-map_option (C11_TypeSpec_2_CleanTyp.conv_GlobalIdDescr_typ o #3) (lookup_Cid_info env_expr "y" );
-\<close>
 
 section \<open>Tests on Expressions\<close>
 
@@ -169,7 +16,6 @@ ML\<open>val ast_expr = @{C11_CExpr}
    val mt_A_env = []
 \<close>
 
-ML\<open>abstract_over\<close>
 
 ML\<open>
 open C11_Expr_2_Clean HOLogic;
@@ -180,6 +26,12 @@ val S = (C11_Ast_Lib.fold_cExpression (K I)
 val S = conv_Cexpr_lifted_term  sigma_i mt_A_env @{theory} ast_expr
 
 \<close>
+
+\<comment> \<open>pretty print of the latter\<close>
+ML\<open>writeln (Syntax.string_of_term_global @{theory} S);\<close>
+
+\<comment> \<open>type-check of the latter\<close>
+ML\<open> Sign.certify_term @{theory} S \<close>
 
 (*2*****************************************************************************************************)
 
@@ -200,6 +52,12 @@ val S = conv_Cexpr_lifted_term  sigma_i mt_A_env @{theory} ast_expr
 
 \<close>
 
+\<comment> \<open>pretty print of the latter\<close>
+ML\<open>writeln (Syntax.string_of_term_global @{theory} S);\<close>
+
+\<comment> \<open>type-check of the latter\<close>
+ML\<open> Sign.certify_term @{theory} S \<close>
+
 (*3*****************************************************************************************************)
 
 (*char :*)
@@ -211,13 +69,17 @@ ML\<open>val ast_expr = @{C11_CExpr}
 \<close>
 
 ML\<open>
-
 val S = (C11_Ast_Lib.fold_cExpression (K I) 
                                       (convertExpr false sigma_i  mt_A_env @{theory}) 
                                       ast_expr []);
 val S = conv_Cexpr_lifted_term  sigma_i mt_A_env @{theory} ast_expr
-
 \<close>
+
+\<comment> \<open>pretty print of the latter\<close>
+ML\<open>writeln (Syntax.string_of_term_global @{theory} S);\<close>
+
+\<comment> \<open>type-check of the latter\<close>
+ML\<open> Sign.certify_term @{theory} S \<close>
 
 (*4*****************************************************************************************************)
 
@@ -238,6 +100,14 @@ val S = conv_Cexpr_lifted_term  sigma_i mt_A_env @{theory} ast_expr
 
 \<close>
 
+ML\<open>@{term "2.997924587"}\<close>
+
+\<comment> \<open>pretty print of the latter\<close>
+ML\<open>writeln (Syntax.string_of_term_global @{theory} S);\<close>
+
+\<comment> \<open>type-check of the latter\<close>
+ML\<open> Sign.certify_term @{theory} S \<close>
+
 (*5*****************************************************************************************************)
 
 
@@ -254,6 +124,12 @@ val S = (C11_Ast_Lib.fold_cExpression (K I)
 val S = conv_Cexpr_lifted_term  sigma_i mt_A_env @{theory} ast_expr
 
 \<close>
+
+\<comment> \<open>pretty print of the latter\<close>
+ML\<open>writeln (Syntax.string_of_term_global @{theory} S);\<close>
+
+\<comment> \<open>type-check of the latter\<close>
+ML\<open> Sign.certify_term @{theory} S \<close>
 
 (*6*****************************************************************************************************)
 
@@ -294,6 +170,12 @@ val S'' = conv_Cexpr_lifted_term  sigma_i A_env2 @{theory} ast_expr
 
 \<close>
 
+\<comment> \<open>pretty print of the latter\<close>
+ML\<open>writeln (Syntax.string_of_term_global @{theory} S);\<close>
+
+\<comment> \<open>type-check of the latter\<close>
+ML\<open> Sign.certify_term @{theory} S \<close>
+
 
 (*7*****************************************************************************************************)
 
@@ -311,6 +193,12 @@ val S = (C11_Ast_Lib.fold_cExpression (K I)
 val S = conv_Cexpr_lifted_term  sigma_i A_env0 @{theory} ast_expr
 
 \<close>
+
+\<comment> \<open>pretty print of the latter\<close>
+ML\<open>writeln (Syntax.string_of_term_global @{theory} S);\<close>
+
+\<comment> \<open>type-check of the latter\<close>
+ML\<open> Sign.certify_term @{theory} S \<close>
 
 section \<open>statements\<close>
 
@@ -342,16 +230,18 @@ val [S] =  (C11_Ast_Lib.fold_cStatement
                 []        \<comment> \<open>mt stack\<close>); 
 \<close>
 
-ML\<open>S\<close>
 \<comment> \<open>pretty print of the latter\<close>
 ML\<open>writeln (Syntax.string_of_term_global @{theory} S);\<close>
+
+\<comment> \<open>type-check of the latter\<close>
+ML\<open> Sign.certify_term @{theory} S \<close>
 
 (*2*****************************************************************************************************)
 
 (*if the body is empty, then we put a skip :*)
 
 C\<open>
-while(1){a = a+1;}
+while(1==1){a = a+1;}
 \<close>
 ML\<open>val ast_stmt = @{C11_CStat}
    val env_stmt = @{C\<^sub>e\<^sub>n\<^sub>v}\<close>
@@ -365,8 +255,11 @@ val [S] =  (C11_Ast_Lib.fold_cStatement
                 ast_stmt  \<comment> \<open>C11 ast\<close>
                 []        \<comment> \<open>mt stack\<close>); 
 \<close>
-\<comment> \<open>Clean pretty print of the latter\<close>
+\<comment> \<open>pretty print of the latter\<close>
 ML\<open>writeln (Syntax.string_of_term_global @{theory} S);\<close>
+
+\<comment> \<open>type-check of the latter\<close>
+ML\<open> Sign.certify_term @{theory} S \<close>
 
 (*3*****************************************************************************************************)
 
@@ -386,8 +279,11 @@ val [S] =  (C11_Ast_Lib.fold_cStatement
                 ast_stmt  \<comment> \<open>C11 ast\<close>
                 []        \<comment> \<open>mt stack\<close>); 
 \<close>
-\<comment> \<open>Clean pretty print of the latter\<close>
+\<comment> \<open>pretty print of the latter\<close>
 ML\<open>writeln (Syntax.string_of_term_global @{theory} S);\<close>
+
+\<comment> \<open>type-check of the latter\<close>
+ML\<open> Sign.certify_term @{theory} S \<close>
 
 (*4*****************************************************************************************************)
 
@@ -410,8 +306,11 @@ val [S] =  (C11_Ast_Lib.fold_cStatement
                 ast_stmt  \<comment> \<open>C11 ast\<close>
                 []        \<comment> \<open>mt stack\<close>); 
 \<close>
-\<comment> \<open>Clean pretty print of the latter\<close>
+\<comment> \<open>pretty print of the latter\<close>
 ML\<open>writeln (Syntax.string_of_term_global @{theory} S);\<close>
+
+\<comment> \<open>type-check of the latter\<close>
+ML\<open> Sign.certify_term @{theory} S \<close>
 
 
 (*5*****************************************************************************************************)
@@ -420,7 +319,7 @@ ML\<open>writeln (Syntax.string_of_term_global @{theory} S);\<close>
 
 (* This local variable space also creates the update function for the return_result. *)
 local_vars_test  (test_return "int")
-    a  :: "int"
+    b  :: "int"
 
 C\<open>
 for(a = 0; a < 10; a = a + 1){
@@ -430,7 +329,9 @@ for(a = 0; a < 10; a = a + 1){
   return a;
 }
 \<close>
-ML\<open>val ast_stmt = @{C11_CStat}\<close>
+ML\<open>val ast_stmt = @{C11_CStat} \<close>
+ML\<open>StateMgt.get_state_field_tab_global @{theory}\<close>
+ML\<open>val sigma_i = StateMgt.get_state_type_global @{theory}\<close>
 
 
 ML\<open>
@@ -441,9 +342,11 @@ val [S] =  (C11_Ast_Lib.fold_cStatement
                 ast_stmt  \<comment> \<open>C11 ast\<close>
                 []        \<comment> \<open>mt stack\<close>); 
 \<close>
-\<comment> \<open>Clean pretty print of the latter\<close>
+\<comment> \<open>pretty print of the latter\<close>
 ML\<open>writeln (Syntax.string_of_term_global @{theory} S);\<close>
-(* the result is structurally incorrect. Where does the if come from ? *)
+
+\<comment> \<open>type-check of the latter\<close>
+ML\<open> Sign.certify_term @{theory} S \<close>
 
 (*following : unfinished work.*)
 
