C11-BackEnds/Clean_wrapper/examples/Coder_Test_Env_AEnv.thy
@@ -1,0 +1,160 @@
+theory "Coder_Test_Env_AEnv"
+  imports "../src/CleanCoder"
+begin
+
+
+
+section \<open>Accessors to C-Env\<close>
+
+ML\<open>
+fun map_option f (SOME X) = SOME(f X)
+   |map_option f NONE     = NONE   
+
+fun lookup_Cid_info (C_env:C_Module.Data_In_Env.T) id = Symtab.lookup(#idents(#var_table C_env)) id
+
+fun is_global_Cid Cenv Cid     = map_option (#global o #3) (lookup_Cid_info Cenv Cid);
+fun is_fun_Cid Cenv Cid        = map_option ((fn [C_Ast.CFunDeclr0 _] => true | _ => false) 
+                                               o (#params o #3)) 
+                                            (lookup_Cid_info Cenv Cid);
+fun get_CDeclSpecS_Cid Cenv id = map_option (#ret o #3) (lookup_Cid_info Cenv id);
+
+(* Fundsachen *)
+C11_Ast_Lib.encode_positions;
+C11_Ast_Lib.decode_positions;
+C11_Ast_Lib.toString_abr_string;
+C11_Ast_Lib.toString_nodeinfo;
+
+C_Ast.SS_base
+\<close>
+
+section \<open>Global Variables, Local Variables, and Local Parameters\<close>
+subsection\<open>An Environment Spy\<close>
+
+ML\<open>
+val ENV = Unsynchronized.ref (@{C\<^sub>e\<^sub>n\<^sub>v})
+fun print_env' s _ stack _ env thy =
+  let
+    val () = (ENV:=env; writeln ("ENV " ^ C_Env.string_of env))
+  in thy end
+\<close>
+
+ML\<open>open Position\<close>
+setup \<open>ML_Antiquotation.inline @{binding print_env'}
+                               (Scan.peek (fn _ => Scan.option Args.text)
+                                >> (fn name => ("print_env' "
+                                                ^ (case name of NONE => "NONE"
+                                                              | SOME s => "(SOME \"" ^ s ^ "\")")
+                                                ^ " " ^ ML_Pretty.make_string_fn)))\<close>
+
+subsection\<open>Accessing the C_Env in an Example\<close>
+
+C \<comment> \<open>Nesting ML code in C comments\<close> \<open>
+int a(int b){int c; 
+              return c;
+              /*@@ \<approx>setup \<open>@{print_env'}\<close> */
+              /*@@ highlight */
+             }; 
+                 
+\<close>
+
+
+ML\<open>
+val a_res = lookup_Cid_info (!ENV) "a";
+val b_res = lookup_Cid_info (!ENV) "b";
+val c_res = lookup_Cid_info (!ENV) "c"
+\<close>
+
+
+(* Problematic : *)
+C \<comment> \<open>Nesting ML code in C comments\<close> \<open>
+int a (int b){int b; 
+              return b;
+              /*@@ highlight */
+              /*@@ \<approx>setup \<open>@{print_env'}\<close> */}; 
+                 
+\<close>
+ML\<open>
+lookup_Cid_info (!ENV) "a";
+lookup_Cid_info (!ENV) "b"
+\<close>
+
+
+
+
+
+section \<open>Global Declarations via CEnv and via the Clean API\<close>
+
+text \<open>
+First, we translate the expressions;
+we can have binary operators, unary operators, or constants.
+The attributs can be constantes or variables. 
+In order to simulate the use of variables, we construct a "fake" record local_state
+\<close>
+
+global_vars (test)  (*intern label *)
+            a     :: "int"
+
+(* creation of a global variable Clean state with "a" *)
+ML\<open>val Const(longid_a,Type("fun",[sigma_i, _])) = @{term "a"}; \<close>
+ML\<open>val sigma_i = StateMgt.get_state_type_global @{theory}\<close>
+
+
+(* creation of two declarations with "a" an array and "f" a function *)
+
+declare [[C\<^sub>r\<^sub>u\<^sub>l\<^sub>e\<^sub>0 = "translation_unit"]]
+declare [[C\<^sub>e\<^sub>n\<^sub>v\<^sub>0 = last]]
+
+C\<open> int a[10+12][34][] = 1;
+   short int f(int x [][], long double y)
+     {int y; x=x;
+      /*@@ \<approx>setup \<open>@{print_env'}\<close> */
+      /*@@ highlight */}
+     ;
+      
+\<close>
+
+(* binding the resulting C_Env to env_expr *)
+
+ML\<open>val env_expr : C_Module.Data_In_Env.T =  @{C\<^sub>e\<^sub>n\<^sub>v};\<close>
+
+(* messing around with the C identifier "a" and "f" in the env AFTER the translation unit*)
+ML\<open>
+   val SOME(pos_list,ser,S)    = lookup_Cid_info env_expr "a";
+   val SOME(pos_list',ser',S') = lookup_Cid_info env_expr "f";
+   val NONE = lookup_Cid_info env_expr "x";
+\<close>
+(* handy decompositions *)
+ML\<open>
+
+local open C_Ast C_Env in
+
+   val [CArrDeclr0 (HH,CArrSize0 (_,CBinary0 X),_),
+        CArrDeclr0 (_,CArrSize0  (_,CConst0 Y), _), 
+        CArrDeclr0 (_,CNoArrSize0 Z,_)] = #params S
+   val [CFunDeclr0 (Right([CDecl0 (A,A' as [((Some (CDeclr0 (_,TT,_,_,_)),_),_)],_),
+                           CDecl0 (B,B' as [((Some (CDeclr0 (_,TT',_,_,_)),_),_)],_)],s), _, _)] 
+       = #params S'
+
+
+val [((Some (CDeclr0 (_,s,_,_,_)),_),_)] = A'
+val [((Some (CDeclr0 (_,t,_,_,_)),_),_)] = B'
+
+end
+\<close>
+
+ML\<open>(#ret o #3 o the)(lookup_Cid_info env_expr "f" );\<close>
+
+ML\<open>
+C11_TypeSpec_2_CleanTyp.conv_CDerivedDecl_typ;C_Ast.CFunDeclr0;
+val S = hd ((#params o  #3 o the)(lookup_Cid_info env_expr "f" ));
+val S' = C11_TypeSpec_2_CleanTyp.conv_CDerivedDecl_typ [S] sigma_i
+\<close>
+(* and the whole thing a bit more abstract with "a" and "f" *)
+ML\<open>
+map_option (C11_TypeSpec_2_CleanTyp.conv_GlobalIdDescr_typ o #3) (lookup_Cid_info env_expr "a" );
+(* map_option (conv_GlobalIdDescr_typ o #3) (lookup_Cid_info env_expr "f" ); *)
+map_option (C11_TypeSpec_2_CleanTyp.conv_GlobalIdDescr_typ o #3) (lookup_Cid_info env_expr "x" );
+map_option (C11_TypeSpec_2_CleanTyp.conv_GlobalIdDescr_typ o #3) (lookup_Cid_info env_expr "y" );
+\<close>
+
+end
